LeanSts/State.lean
@@ -1,0 +1,11 @@
+-- FIXME: I'm not sure why this is needed
+import Mathlib.Tactic
+
+def updateFn [DecidableEq α] (f : α → β) (a : α) (b : β) : α → β :=
+  λ (x : α) => if x = a then b else f x
+
+notation st"[ " a " ↦ " b " ]" => updateFn st a b
+
+@[simp] lemma updateFn_unfold [DecidableEq α] (f : α → β) (a : α) (b : β) (x : α) :
+  (f[a ↦ b]) x = if x = a then b else f x := by
+  simp only [updateFn]
