lakefile.lean
@@ -9,8 +9,7 @@ lean_lib «LeanSts» where
 
 lean_lib «Examples» where
 
-require mathlib from git "https://github.com/leanprover-community/mathlib4.git"
-require LSpec from git "https://github.com/lurk-lab/LSpec.git"
+require mathlib from git "https://github.com/leanprover-community/mathlib4.git" @ "v4.6.0-rc1"
 
 @[default_target]
 lean_exe «lean-sts» where
